\begin{lemma}[Substitution]
  \lbl{lem:substitution}~
  \begin{enumerate}
    \item % 0
    If $\Γ, \X \<: \Q, \Δ \⊢ \disj(\S, \T)$ and $\Γ \⊢ \P \<: \Q$,
    then $\Γ, \[\X \↦ \P] \Δ \⊢ \disj(\[\X \↦ \P] \S, \[\X \↦ \P] \T)$.

    \item % 1
    If $\Γ, \X \<: \Q, \Δ \⊢ \S \<: \T$ and $\Γ \⊢ \P \<: \Q$,
    then $\Γ, \[\X \↦ \P] \Δ \⊢ \[\X \↦ \P] \S \<: \[\X \↦ \P] \T$.

    \item % 2
    If $\Γ, \X \<: \Q, \Δ \⊢ \t \: \T$ and $\Γ \⊢ \P \<: \Q$,
    then $\Γ, \[\X \↦ \P] \Δ \⊢ \[\X \↦ \P] \t \: \[\X \↦ \P] \T$.

    \item % 3
    If $\Γ, \x \: \Q, \Δ \⊢ \t \: \T$ and $\Γ \⊢ \q \: \Q$,
    then $\Γ, \Δ \⊢ \[\x \↦ \q] \t \: \T$.
  \end{enumerate}
\end{lemma}

\begin{proof}
  We prove 1. and 2. simultaneously by induction on two derivations of $\Γ, \X \<: \Q, \Δ \⊢ \disj(\V, \W)$ and $\Γ, \X \<: \Q, \Δ \⊢ \S \<: \T$.
  More precisely, the induction is done on the cumulative depth of both derivation tree.
  \begin{enumerate}
    \item % 0
    $\Γ, \X \<: \Q, \Δ \⊢ \disj(\V, \W)$
    \begin{itemize}
      \Case\DXi:
      \quad $\V \= \C_{1}$
      \quad $\W \= \C_{2}$
      \quad $\(\C_{1}, \C_{2}) \∈ \Ξ$

      Since $\[\X \↦ \P] \C_{1} \= \C_{1}$ and $\[\X \↦ \P] \C_{2} \= \C_{2}$, we can use \DXi with context $\Γ, \[\X \↦ \P] \Δ$ to obtain the desired result.

      \Case\DPsi:
      \quad $\V \= \{ \new \C_{1} \}$
      \quad $\W \= \C_{2}$
      \quad $\(\C_{1}, \C_{2}) \∉ \Ψ$

      Since $\[\X \↦ \P] \{ \new \C_{1} \} \= \{ \new \C_{1} \}$ and $\[\X \↦ \P] \C_{2} \= \C_{2}$, we can use \DPsi with context $\Γ, \[\X \↦ \P] \Δ$ to obtain the desired result.

      \Case\DSub:
      \quad $\Γ, \X \<: \Q, \Δ \⊢ \V \<: \U$
      \quad $\Γ, \X \<: \Q, \Δ \⊢ \disj(\U, \W)$

      By the IH we get $\Γ, \[\X \↦ \P] \Δ \⊢ \disj(\[\X \↦ \P] \U, \[\X \↦ \P] \W)$.
      Using the 2nd part of the lemma we obtain $\Γ, \[\X \↦ \P] \Δ \⊢ \[\X \↦ \P] \V \<: \[\X \↦ \P] \U$.
      The result follows from \DSub.

      \Case\DArrow:
      \quad $\V \= \V_{1} \→ \V_{2}$
      \quad $\W \= \C$

      Since $\[\X \↦ \P] \(\V_{1} \→ \V_{2}) \= \[\X \↦ \P] \V_{1} \→ \[\X \↦ \P] \V_{2}$ and $\[\X \↦ \P] \C \= \C$,
      we can use \DArrow with context $\Γ, \[\X \↦ \P] \Δ$ to obtain the desired result.

      \Case\DAll:
      \quad $\V \= \∀ \Y \<: \V_{1}.~ \V_{2}$
      \quad $\W \= \C$

      Since $\[\X \↦ \P] \(\∀ \Y \<: \V_{1}.~ \V_{2}) \= \∀ \Y \<: \[\X \↦ \P] \V_{1}.~ \[\X \↦ \P] \V_{2}$ and $\[\X \↦ \P] \C \= \C$,
      we can use \DAll with context $\Γ, \[\X \↦ \P] \Δ$ to obtain the desired result.
    \end{itemize}

    \item % 1
    $\Γ, \X \<: \Q, \Δ \⊢ \S \<: \T$.
    \begin{itemize}
      \Case\SRefl:
      \quad $\T \= \S$

      The result follows directly from \SRefl.

      \Case\STrans:
      \quad $\Γ, \X \<: \Q, \Δ \⊢ \S \<: \U$
      \quad $\Γ, \X \<: \Q, \Δ \⊢ \U \<: \T$

      The result follows directly from the IH and \STrans.

      \Case\STop:
      \quad $\T \= \Top$

      $\[\X \↦ \P] \Top \= \Top$ and the result follows from \STop.

      \Case\SSin:
      \quad $\S \= \{ \new \C \}$
      \quad $\T \= \C$

      $\[\X \↦ \P] \{ \new \C \} \= \{ \new \C \}$,
      $\[\X \↦ \P] \C \= \C$,
      and the result follows from \SSin.

      \Case\STvar:
      \quad $\S \= \Y$
      \quad $\Y \<: \T \∈ \(\Γ, \X \<: \Q, \Δ)$

      By context well-formedness, $\Y \<: \T \∈ \(\Γ, \X \<: \Q, \Δ)$ can be decomposed into 3 subcases:
      \begin{itemize}
        \Subcase $\Y \<: \T \∈ \Γ$:

        By context well-formedness $\X$ does not appear in $\Γ$ consequently is also absent from $\Y$ and $\T$.
        Hence $\Y \= \[\X \↦ \P] \Y$, $\T \= \[\X \↦ \P] \T$ and $\[\X \↦ \P] \Y \<: \[\X \↦ \P] \T \∈ \(\Γ, \[\X \↦ \P] \Δ)$.
        The result follows from \STvar.

        \Subcase $\Y \<: \T \∈ \Δ$:

        $\[\X \↦ \P] \Y \<: \[\X \↦ \P] \T \∈ \[\X \↦ \P] \Δ$ and $\[\X \↦ \P] \Y \<: \[\X \↦ \P] \T \∈ \(\Γ, \[\X \↦ \P] \Δ)$. The result follows from \STvar.

        \Subcase $\Y \<: \T \= \X \<: \Q$ (\emph{i.e.} $\Y \= \X$ and $\T \= \Q$):

        By context well-formedness, $\X$ doesn't appear in $\Q$, and $\[\X \↦ \P] \T \= \[\X \↦ \P] \Q \= \Q$.
        Also $\[\X \↦ \P] \S \= \[\X \↦ \P] \X \= \P$ and $\[\X \↦ \P] \T \= \Q$.
        As a result, $\Γ \⊢ \P \<: \Q$ implies $\Γ \⊢ \[\X \↦ \P] \S \<: \[\X \↦ \P] \T$.
        Using \Cref{lem:weakening} we get $\Γ, \[\X \↦ \P] \Δ \⊢ \[\X \↦ \P] \S \<: \[\X \↦ \P] \T$, as required.

      \end{itemize}

      \Case\SArrow:
      \quad $\S \= \S_{1} \→ \S_{2}$
      \quad $\T \= \T_{1} \→ \T_{2}$
      \\\phantom{\textit{Case}~\SArrow:}
      \quad $\Γ, \X \<: \Q, \Δ \⊢ \T_{1} \<: \S_{1}$
      \quad $\Γ, \X \<: \Q, \Δ \⊢ \S_{2} \<: \T_{2}$

      $\[\X \↦ \P] \(\S_{1} \→ \S_{2}) \= \[\X \↦ \P] \S_{1} \→ \[\X \↦ \P] \S_{2}$,
      $\[\X \↦ \P] \(\T_{1} \→ \T_{2}) \= \[\X \↦ \P] \T_{1} \→ \[\X \↦ \P] \T_{2}$.
      The result follows from the IH and \SArrow.

      \Case\SAll:
      \quad $\S \= \∀ \Y \<: \U_{1}.~ \S_{2}$
      \quad $\T \= \∀ \Y \<: \U_{1}.~ \T_{2}$
      \quad $\Γ, \X \<: \Q, \Δ, \Y \<: \U_{1} \⊢ \S_{2} \<: \T_{2}$

      We instantiate the IH with $\Δ_{IH} \= \(\Δ, \Y \<: \U_{1})$ to obtain
      $\Γ, \[\X \↦ \P] \Δ, \Y \<: \[\X \↦ \P] \U_{1} \⊢ \[\X \↦ \P] \S_{2} \<: \[\X \↦ \P] \T_{2}$.
      Using \SAll, we get
      $\Γ, \[\X \↦ \P] \Δ \⊢ \(\∀ \Y \<: \[\X \↦ \P] \U_{1}.~ \[\X \↦ \P] \S_{2}) \<: \(\∀ \Y \<: \[\X \↦ \P] \U_{1}.~ \[\X \↦ \P] \T_{2})$, that is,
      $\Γ, \[\X \↦ \P] \Δ \⊢ \[\X \↦ \P] \(\∀ \Y \<: \U_{1}.~ \S_{2}) \<: \[\X \↦ \P] \(\∀ \Y \<: \U_{1}.~ \T_{2})$, as required.

      \Case\SPsi:
      \quad $\S \= \C_{1}$
      \quad $\T \= \C_{2}$
      \quad $\(\C_{1}, \C_{2}) \∈ \Ψ$

      $\[\X \↦ \P] \C_{1} \= \C_{1}$ and $\[\X \↦ \P] \C_{2} \= \C_{2}$. The result follows from \SPsi.

      \Case\SMatch1/2:
      \quad $\T_{1} \= \T_n$
      \quad $\T_{2} \= \T_s \match \{ \S_i \⇒ \T_i \} \otherwise \T_d$
      \\\phantom{\textit{Case}~\SMatch1/2:}
      \quad $\Γ, \X \<: \Q, \Δ \⊢ \T_s \<: \S_n$
      \quad $\∀ \m<n.~ \Γ, \X \<: \Q, \Δ \⊢ \disj(\T_s, \S_m)$

      Using the 1st part of the lemma we get $\∀ \m< \n.~ \Γ, \[\X \↦ \P] \Δ \⊢ \disj(\[\X \↦ \P] \T_s, \[\X \↦ \P] \S_m)$.
      By the IH we get $\Γ, \[\X \↦ \P] \Δ \⊢ \[\X \↦ \P] \T_s \<: \S_n$.
      $\[\X \↦ \P] \T \= \[\X \↦ \P] \T_s \match \{$ $\[\X \↦ \P] \S_i \⇒ \[\X \↦ \P] \T_i \} \otherwise \[\X \↦ \P] \T_d$,
      and the result follows from \SMatch1/2.

      \Case\SMatch3/4:
      \quad $\S \= \T_d$
      \quad $\T \= \T_s \match \{ \S_i \⇒ \T_i \} \otherwise \T_d$
      \\\phantom{\textit{Case}~\SMatch1/2:}
      \quad $\∀ \n.~ \Γ, \X \<: \Q, \Δ \⊢ \disj(\T_s, \S_n)$

      By the 1st part of the lemma we get $\∀ \n.~ \Γ, \[\X \↦ \P] \Δ \⊢ \disj(\[\X \↦ \P] \T_s, \[\X \↦ \P] \S_n)$ and the result follows from \SMatch3/4.

      \Case\SMatch5:
      \quad $\S \= \S_s \match \{ \U_i \⇒ \S_i \} \otherwise \S_d$
      \quad $\T \= \T_s \match \{ \U_i \⇒ \T_i \} \otherwise \T_d$
      \\\phantom{\textit{Case}~\SMatch5:}
      \quad $\Γ, \X \<: \Q, \Δ \⊢ \S_s \<: \T_s$
      \quad $\∀ \n.~ \Γ, \X \<: \Q, \Δ \⊢ \S_n \<: \T_n$
      \\\phantom{\textit{Case}~\SMatch5:}
      \quad $\Γ, \X \<: \Q, \Δ \⊢ \S_d \<: \T_d$

      The result follows directly from the IH.
    \end{itemize}

    % 2
    \item By induction on a derivation of $\Γ, \X \<: \Q, \Δ \⊢ \t \: \T$.
    \begin{itemize}
        \Case\TVar:
        \quad $\t \= \x$
        \quad $\x \: \T \∈ \Γ, \X \<: \Q, \Δ$

        $\[\X \↦ \P] \x \= \x$. \TVar's premise can be divided in two subcases:
        \begin{itemize}
          \Subcase $\x \: \T \∈ \Γ$:

          Context well-formedness impiles that there is no occurence of $\X$ in $\T$ and $\[\X \↦ \P] \T \= \T$.
          Also, $\x \: \T \∈ \Γ, \[\X \↦ \P] \Δ$ and the result follows from \TVar.

          \Subcase $\x \: \T \∈ \Δ$:

          Context well-formedness impiles that there is a unique occurence of $\x \: \T$ in $\Δ$, that is,
          there exists $\Δ_1$, $\Δ_2$ such that $\Δ \= \Δ_1, \x \: \T, \Δ_2$, $\x \not \in \Δ_1$ and $\x \not \in \Δ_2$.
          As a result, $\[\X \↦ \P] \Δ$ = $\[\X \↦ \P] \Δ_1, \x \: \[\X \↦ \P] \T, \[\X \↦ \P] \Δ_2$
          and $\x \: \[\X \↦ \P] \T \∈ \Γ, \[\X \↦ \P] \Δ$.
          The result follows from \TVar.
        \end{itemize}

        \Case\TAbs:
        \quad $\t \= \λ \x \: \T_{1} \t_{2}$
        \quad $\T \= \T_{1} \→ \T_{2}$
        \quad $\Γ, \X \<: \Q, \Δ, \x \: \T_{1} \⊢ \t_{2} \: \T_{2}$

        $\[\X \↦ \P] \(\λ \x \: \T_{1} \t_{2}) \= \λ \x \: \[\X \↦ \P] \T_{1} \[\X \↦ \P] \t_{2}$ and
        $\[\X \↦ \P] \(\T_{1} \→ \T_{2}) \= \[\X \↦ \P] \T_{1} \→ \[\X \↦ \P] \T_{2}$.
        We instantiate the IH with $\Δ_{IH} \= \(\Δ, \x \: \T_{1})$ to obtain\\
        $\Γ, \[\X \↦ \P] \Δ, \x \: \[\X \↦ \P] \T_{1} \⊢ \[\X \↦ \P] \t_{2} \: \[\X \↦ \P] \T_{2}$.
        The result follows from \TAbs.

        \Case\TApp:
        \quad $\t \= \t_{1} \t_{2}$
        \quad $\T \= \T_{12}$
        \quad $\Γ, \X \<: \Q, \Δ \⊢ \t_{1} \: \T_{11} \→ \T_{12}$
        \quad $\Γ, \X \<: \Q, \Δ \⊢ \t_{2} \: \T_{11}$

        $\[\X \↦ \P] \(\t_{1} \t_{2}) \= \[\X \↦ \P] \t_{1} \[\X \↦ \P] \t_{2}$,
        $\[\X \↦ \P] \T_{11} \→ \T_{12} \= \[\X \↦ \P] \T_{11} \→ \[\X \↦ \P] \T_{12}$.
        The result follows directly from the IH and \TApp.

        \Case\TTAbs:
        \quad $\t \= \λ \Y \<: \T_{1}.~ \t_{2}$
        \quad $\T \= \∀ \Y \<: \T_{1}.~ \T_{2}$
        \quad $\Γ, \X \<: \Q, \Δ, \Y \<: \T_{1} \⊢ \t_{2} \: \T_{2}$

        $\[\X \↦ \P] \(\λ \Y \<: \T_{1}.~ \t_{2}) \= \λ \Y \<: \[\X \↦ \P] \T_{1}.~ \[\X \↦ \P] \t_{2}$ and
        $\[\X \↦ \P] \(\∀ \Y \<: \T_{1}.~ \T_{2}) \= \∀ \Y \<: \[\X \↦ \P] \T_{1}.~ \[\X \↦ \P] \T_{2}$.
        We instantiate the IH with $\Δ_{IH} \= \(\Δ, \Y \<: \T_{1})$ to obtain
        $\Γ, \[\X \↦ \P] \Δ, \Y \<: \[\X \↦ \P] \T_{1} \⊢ \[\X \↦ \P] \t_{2} \: \[\X \↦ \P] \T_{2}$.
        The result follows from \TTAbs.

        \Case\TTApp:
        \quad $\t \= \t_{1} \T_{2}$
        \quad $\T \= \[\Y \↦ \T_{2}] \T_{12}$
        \\\phantom{\textit{Case}~\TTApp:}
        \quad $\Γ, \X \<: \Q, \Δ \⊢ \t_{1} \: \(\∀ \Y \<: \T_{11}.~ \T_{12})$
        \quad $\Γ, \X \<: \Q, \Δ \⊢ \T_{2} \<: \T_{11}$

        By the IH,
        $\Γ, \[\X \↦ \P] \Δ \⊢ \[\X \↦ \P] \t_{1} \: \[\X \↦ \P] \(\∀ \Y \<: \T_{11}.~ \T_{12})$, i.e.,
        $\Γ, \[\X \↦ \P] \Δ \⊢ \[\X \↦ \P] \t_{1} \: \∀ \Y \<: \[\X \↦ \P] \T_{11}.~ \[\X \↦ \P] \T_{12}$.
        Using the second part of the lemma we get,
        $\Γ, \[\X \↦ \P] \Δ \⊢ \[\X \↦ \P] \T_{2} \<: \[\X \↦ \P] \T_{11}$.
        By \TTApp we get,
        $\Γ, \[\X \↦ \P] \Δ \⊢ \[\X \↦ \P] \t_{1} \[\X \↦ \P] \T_{2} \: \[\Y \↦ \[\X \↦ \P] \T_{2}] \[\X \↦ \P] \T_{12}$, i.e.,
        $\Γ, \[\X \↦ \P] \Δ \⊢ \[\X \↦ \P] \(\t_{1} \T_{2}) \: \[\X \↦ \P](\[\Y \↦ \T_{2}] \T_{12})$, as required.

        \Case\TSub:
        \quad $\Γ, \X \<: \Q, \Δ \⊢ \t \: \S$
        \quad $\Γ, \X \<: \Q, \Δ \⊢ \S \<: \T$

        By the IH, $\Γ, \[\X \↦ \P] \Δ \⊢ \[\X \↦ \P] \t \: \[\X \↦ \P] \S$.
        Using the second part of the lemma we get,
        $\Γ, \[\X \↦ \P] \Δ \⊢ \[\X \↦ \P] \S \<: \[\X \↦ \P] \T$.
        The result follows from \TSub.

        \Case\TClass:
        \quad $\t \= \new \C$
        \quad $\T \= \{ \new \C \}$

        $\[\X \↦ \P] \new \C \= \new \C$ and using \TClass with context $\Γ, \[\X \↦ \P] \Δ$ directly leads to the desired result.

        \Case\TMatch:
        \quad $\t \= \t_s \match \{ \x_i \: \C_i \⇒ \t_i \} \otherwise \t_d$
        \quad $\T \= \T_s \match \{ \C_i \⇒ \T_i \} \otherwise \T_d$
        \\\phantom{\textit{Case}~\TMatch:}
        \quad $\Γ, \X \<: \Q, \Δ \⊢ \t_s \: \T_s$
        \quad $\Γ, \X \<: \Q, \Δ, \x_i \: \C_i \⊢ \t_i \: \T_i$
        \\\phantom{\textit{Case}~\TMatch:}
        \quad $\Γ, \X \<: \Q, \Δ \⊢ \t_d \: \T_d$

        $\[\X \↦ \P] \(\t_s \match \{ \x_i \: \C_i \⇒ \t_i \} \otherwise \t_d) \= \[\X \↦ \P] \t_s \match \{ \x_i \: \C_i \⇒ \[\X \↦ \P] \t_i \} \otherwise \[\X \↦ \P] \t_d$.

        $\[\X \↦ \P] \(\T_s \match \{ \C_i \⇒ \T_i \} \otherwise \T_d) \= \[\X \↦ \P] \T_s \match \{ \C_i \⇒ \[\X \↦ \P] \T_i \} \otherwise \[\X \↦ \P] \T_d$.

        The result follows directly from the IH and \TApp.
    \end{itemize}

    \item % 3
    By induction on a derivation of $\Γ, \x \: \Q, \Δ \⊢ \t \: \T$.
    \begin{itemize}
      \Case\TVar:
      \quad $\t \= \y$
      \quad $\y \: \T \∈ \Γ, \x \: \Q, \Δ$

      By context well-formedness, the premise can be decomposed into 3 subcases:

      \begin{itemize}
        \Subcase $\y \: \T \∈ \Γ$:

        $\[\x \↦ \q] \y \= \y$ and $\y \: \T \∈ \Γ, \Δ$. The result follows from \TVar.

        \Subcase $\y \: \T \∈ \Δ$:

        Ditto.

        \Subcase $\y \: \T \= \x \: \Q$ (i.e. $\y \= \x$ and $\T \= \Q$):

        Using $\Γ \⊢ \q \: \Q$ and \Cref{lem:weakening} we get $\Γ, \Δ \⊢ \q \: \Q$. Since $\[\x \↦ \q] \y \= \q$ and $\T \= \Q$, $\Γ, \Δ \⊢ \[\x \↦ \q] \y \: \T$, as required.

      \end{itemize}

      \Case\TAbs:
      \quad $\t \= \λ \y \: \T_{1} \t_{2}$
      \quad $\T \= \T_{1} \→ \T_{2}$
      \quad $\Γ, \x \: \Q, \Δ, \y \: \T_{1} \⊢ \t_{2} \: \T_{2}$

      We instantiate the IH with $\Δ_{IH} \= \(\Δ, \y \: \T_{1})$ to obtain $\Γ, \Δ, \y \: \T_{1} \⊢ \[\x \↦ \q] \t_{2} \: \T_{2}$.
      $\[\x \↦ \q] \(\λ \y \: \T_{1} \t_{2}) \= \λ \y \: \T_{1} \[\x \↦ \q] \t_{2}$ and the result follows from \TAbs.

      \Case\TApp:
      \quad $\t \= \t_{1} \t_{2}$
      \quad $\T \= \T_{12}$
      \quad $\Γ, \x \: \Q, \Δ \⊢ \t_{1} \: \T_{11} \→ \T_{12}$
      \quad $\Γ, \x \: \Q, \Δ \⊢ \t_{2} \: \T_{11}$

      $\[\x \↦ \q] \(\t_{1} \t_{2}) \= \(\[\x \↦ \q] \t_{1}) \(\[\x \↦ \q] \t_{2})$ and the result follows from the IH and \TApp.

      \Case\TTAbs:
      \quad $\t \= \λ \X \<: \U_{1}.~ \t_{2}$
      \quad $\T \= \∀ \X \<: \U_{1}.~ \T_{2}$
      \quad $\Γ, \x \: \Q, \Δ, \X \<: \U_{1} \⊢ \t_{2} \: \T_{2}$

      We instantiate the IH with $\Δ_{IH} \= \(\Δ, \X \<: \U_{1})$ to obtain $\Γ, \Δ, \X \<: \U_{1} \⊢ \[\x \↦ \q] \t_{2} \: \T_{2}$.
      $\[\x \↦ \q] \(\λ \X \<: \U_{1}.~ \t_{2}) \= \λ \X \<: \U_{1}.~ \[\x \↦ \q] \t_{2}$ and the result follows from \TTAbs.

      \Case\TTApp:
      \quad $\t \= \t_{1} \T_{2}$
      \quad $\T \= \[\X \↦ \T_{2}] \T_{12}$
      \\\phantom{\textit{Case}~\TTApp:}
      \quad $\Γ, \x \: \Q, \Δ \⊢ \t_{1} \: \(\∀ \X \<: \U_{1}.~ \T_{12})$
      \quad $\Γ, \x \: \Q, \Δ \⊢ \T_{2} \<: \U_{1}$

      By \Cref{lem:strengthening}, $\Γ, \Δ \⊢ \T_{2} \<: \U_{1}$.
      From the IH we get $\Γ, \Δ \⊢ \[\x \↦ \q] \t_{1} \: \(\∀ \X \<: \U_{1}.~ \T_{12})$.
      $\[\x \↦ \q] \(\t_{1} \T_{2}) \= \[\x \↦ \q] \t_{1} \T_{2}$ and the result follows from \TTApp.

      \Case\TSub:
      \quad $\Γ, \x \: \Q, \Δ \⊢ \t \: \S$
      \quad $\Γ, \x \: \Q, \Δ \⊢ \S \<: \T$

      By \Cref{lem:strengthening}, $\Γ, \Δ \⊢ \S \<: \T$. The result follows from the IH and \TSub.

      \Case\TClass:
      \quad $\t \= \new \C$
      \quad $\T \= \{ \new \C \}$

      Since $\[\x \↦ \q] \new \C \= \new \C$, using \TClass with context $\Γ, \Δ$ directly leads to the desired result.

      \Case\TMatch:
      \quad $\t \= \t_s \match \{ \x_i \: \C_i \⇒ \t_i \} \otherwise \t_d$
      \quad $\T \= \T_s \match \{ \C_i \⇒ \T_i \} \otherwise \T_d$
      \\\phantom{\textit{Case}~\TMatch:}
      \quad $\Γ, \x \: \Q, \Δ \⊢ \t_s \: \T_s$
      \quad $\Γ, \x \: \Q, \Δ, \x_i \: \C_i \⊢ \t_i \: \T_i$
      \quad $\Γ, \x \: \Q, \Δ \⊢ \t_d \: \T_d$

      $\[\x \↦ \q] \(\t_s \match \{ \x_i \: \C_i \⇒ \t_i \} \otherwise \t_d) \= \[\x \↦ \q] \t_s \match \{ \x_i \: \C_i \⇒ \[\x \↦ \q] \t_i \} \otherwise \[\x \↦ \q] \t_d$, and the result follows from the IH and \TMatch.
    \end{itemize}
  \end{enumerate}
\end{proof}
